Gt3/Syntax/Logic.lean
@@ -8,6 +8,10 @@ def Tm.not {k} (φ : Tm k) : Tm k := .eqn φ .empty
 
 def Tm.or {k} (φ ψ : Tm k) : Tm k := .imp (.not φ) ψ
 
+def Tm.forall {k} (A : Tm k) (φ : Tm (k + 1)) : Tm k := .trunc (.pi A φ)
+
+def Tm.exists {k} (A : Tm k) (φ : Tm (k + 1)) : Tm k := .trunc (.sigma A φ)
+
 @[simp]
 theorem Tm.open_imp {k} (φ ψ : Tm (k + 1)) (x : String)
   : (φ.imp ψ).open x = (φ.open x).imp (ψ.open x) := by simp [imp]
@@ -23,3 +27,37 @@ theorem Tm.open_not {k} (φ : Tm (k + 1)) (x : String)
 @[simp]
 theorem Tm.open_or {k} (φ ψ : Tm (k + 1)) (x : String)
   : (φ.or ψ).open x = (φ.open x).or (ψ.open x) := by simp [or]
+
+@[simp]
+theorem Tm.open_forall {k} (A : Tm (k + 1)) (φ : Tm (k + 2)) (x : String)
+  : (A.forall φ).open x = (A.open x).forall (φ.open x) := by simp [«forall»]
+
+@[simp]
+theorem Tm.open_exists {k} (A : Tm (k + 1)) (φ : Tm (k + 2)) (x : String)
+  : (A.exists φ).open x = (A.open x).exists (φ.open x) := by simp [«exists»]
+
+@[simp]
+theorem Tm.smul_imp (v : VSubst) {k} (φ ψ : Tm k) : v • (φ.imp ψ) = (v • φ).imp (v • ψ)
+  := by simp [imp]
+
+@[simp]
+theorem Tm.smul_and (v : VSubst) {k} (φ ψ : Tm k) : v • (φ.and ψ) = (v • φ).and (v • ψ)
+  := by simp [and]
+
+@[simp]
+theorem Tm.smul_not (v : VSubst) {k} (φ : Tm k) : v • φ.not = (v • φ).not
+  := by simp [not]
+
+@[simp]
+theorem Tm.smul_or (v : VSubst) {k} (φ ψ : Tm k) : v • (φ.or ψ) = (v • φ).or (v • ψ)
+  := by simp [or]
+
+@[simp]
+theorem Tm.smul_forall (v : VSubst) {k} (A : Tm k) (φ : Tm (k + 1))
+  : v • (A.forall φ) = (v • A).forall (v • φ)
+  := by simp [«forall»]
+
+@[simp]
+theorem Tm.smul_exists (v : VSubst) {k} (A : Tm k) (φ : Tm (k + 1))
+  : v • (A.exists φ) = (v • A).exists (v • φ)
+  := by simp [«exists»]
